clean up c_list_zipWith_evp; remove grinds

Computability/Constructions/List.lean
@@ -438,7 +438,7 @@ def c_list_map (cf:Code) := (c_list_foldr (c_list_cons.comp₂ (cf.comp left) ri
 end Nat.RecursiveIn.Code
 end list_map
 
-section list_zip
+section list_zipWith
 namespace Nat.RecursiveIn.Code
 /-
 zipL :: [a] -> [b] -> [(a,b)]
@@ -447,7 +447,7 @@ zipL xs ys = reverse $ fst $ foldl step ([], ys) xs
     step (acc, y:ys') x = ((x,y) : acc, ys')
     step (acc, [])    _ = (acc, [])
 -/
-def c_list_zip :=
+def c_list_zipWith (cf:Code):=
   let yys' := right.comp left
   let ys'  := c_list_tail.comp  yys'
   let y    := c_list_headI.comp yys'
@@ -458,27 +458,15 @@ def c_list_zip :=
     c_list_casesOn'
     yys'
     left
-    (pair (c_list_cons.comp₂ (pair x y) (acc)) ys')
-  -- overall input: (xl,yl)
-  -- so here xl is the accumulator at the start.
-  -- within foldr, our function takes inputs of the form:
-  -- (head of list (y), accumulator)
-  -- `foldr f acc (y:ys) = f y (foldr f acc ys)`
-  -- `foldr f (x:xs) (y:ys) = f y (foldr f (x:xs) ys)`
-  -- `foldr f (x) (y) = f y (foldr f (x) ()))`
-  -- `foldr f (x) () = (x)`
-  -- `foldr f (x) (y) = f y (x)`
+    (pair (c_list_cons.comp₂ (cf.comp₂ x y) (acc)) ys')
 
-  -- we want our final accumulator to be `[(x₀,y₀),...]`
-
-  -- c_list_reverse.comp (left.comp ((c_list_foldl step).comp₂ (pair c_list_nil right) left))
   (c_list_foldl step).comp₂ (pair c_list_nil right) left
 #check List.zipWith
--- #eval eval_prim (Nat.fzero) c_list_zip (Nat.pair [1] [3])
+-- #eval eval_prim (Nat.fzero) c_list_zipWith (Nat.pair [1] [3])
 -- theorem zip_aux : List.foldr () = List.zip ()
-@[simp] theorem c_list_zip_ev_pr : code_prim c_list_zip := by unfold c_list_zip; repeat (first|assumption|simp|constructor)
--- @[simp] theorem c_list_zip_evp : eval_prim O c_list_zip (Nat.pair l1N l2N) = l2n (List.zipWith Nat.pair (n2l l1N) (n2l l2N)) := by
-theorem c_list_zip_evp_aux_2P {a b : List ℕ} {f:ℕ→ℕ→ℕ} (h:a.length≤b.length) : List.zipWith f (b++c) a = List.zipWith f b a := by
+@[simp] theorem c_list_zipWith_ev_pr (hcf:code_prim cf) : code_prim (c_list_zipWith cf) := by unfold c_list_zipWith; repeat (first|assumption|simp|constructor)
+-- @[simp] theorem c_list_zipWith_evp : eval_prim O c_list_zipWith (Nat.pair l1N l2N) = l2n (List.zipWith Nat.pair (n2l l1N) (n2l l2N)) := by
+theorem c_list_zipWith_evp_aux_2 {a b : List ℕ} {f:ℕ→ℕ→ℕ} (h:a.length≤b.length) : List.zipWith f (b++c) a = List.zipWith f b a := by
   have aux3 : b = take a.length (b) ++ drop a.length (b) := by
     exact Eq.symm (take_append_drop a.length (b))
   rw [aux3]
@@ -494,38 +482,51 @@ theorem c_list_zip_evp_aux_2P {a b : List ℕ} {f:ℕ→ℕ→ℕ} (h:a.length�
   have aux8 := @zipWith_append ℕ ℕ ℕ f (take a.length b) (drop a.length b) a [] aux7
   simp at aux8
   rw [aux8]
+theorem zipWith_flip : List.zipWith f a b = List.zipWith (flip f) b a := by
+    induction a generalizing b with
+    | nil => simp
+    | cons x xs xih =>
+      induction b with
+      | nil => simp
+      | cons y ys yih =>
+        simp [xih, flip]
+
+theorem c_list_zipWith_evp_aux_1 {a b : List ℕ} {f:ℕ→ℕ→ℕ} (h:a.length≤b.length) : List.zipWith f a (b++c) = List.zipWith f a b := by
+  rw [zipWith_flip]
+  rw (config:={occs:=.pos [2]}) [zipWith_flip]
+  exact c_list_zipWith_evp_aux_2 h
 
 
-  
-  -- exact?
-  
-@[simp] theorem c_list_zip_evp :
-  eval_prim O c_list_zip (Nat.pair l1N l2N)
+@[simp] theorem c_list_zipWith_evp :
+  eval_prim O (c_list_zipWith cf) (Nat.pair l1N l2N)
     =
-  Nat.pair ((List.zipWith Nat.pair l1N l2N).reverse) (drop (n2l l1N).length (n2l l2N)) := by
-  
-  simp [c_list_zip, -encode_list_cons, -encode_list_nil]
-  have asd: ((n2l l1N).reverse).reverse = (n2l l1N) := by exact reverse_reverse (n2l l1N)
-  -- induction (n2l l1N) with
-  -- induction (n2l l1N).reverse with
+  Nat.pair ((List.zipWith (fun x y => eval_prim O cf (Nat.pair x y)) l1N l2N).reverse) (drop (n2l l1N).length (n2l l2N)) := by
+
+  let f:=fun x y => eval_prim O cf (Nat.pair x y)
+
+  simp [c_list_zipWith, -encode_list_cons, -encode_list_nil]
+  have grind_helper_1: ((n2l l1N).reverse).reverse = (n2l l1N) := by exact reverse_reverse (n2l l1N)
   induction h:(n2l l1N).reverse generalizing l1N with
   | nil => simp_all
   | cons head tail ih =>
-    have asd2 : (n2l l1N) = (tail.reverse).concat head := by grind
-
+    have asd2 : (n2l l1N) = (tail.reverse).concat head := by
+      rw [concat_eq_append]
+      rw [←reverse_reverse (n2l l1N)]
+      rw [h]
+      apply reverse_cons
     rw [asd2]
+
     simp [-encode_list_cons, -encode_list_nil] at ih
-    -- rw [asd] at ih
     have asdd : (n2l (l2n tail.reverse)).reverse = tail := by simp
-    -- simp [ih asdd]
     simp [-encode_list_cons, -encode_list_nil, -foldl_reverse]
     have lolz := ih asdd
     simp [-encode_list_cons, -encode_list_nil, -foldl_reverse] at lolz
     rw [lolz]
     simp [-encode_list_cons, -encode_list_nil, -foldl_reverse]
-    
+
+
     by_cases hh:(drop tail.length (n2l l2N))=([]:List ℕ)
-    · 
+    ·
       simp only [hh]
       have aux1: drop (tail.length + 1) (n2l l2N) = [] := by
         simp
@@ -534,27 +535,30 @@ theorem c_list_zip_evp_aux_2P {a b : List ℕ} {f:ℕ→ℕ→ℕ} (h:a.length�
       have aux4 := List.drop_eq_nil_iff.mp hh
       have aux5 : tail.length = tail.reverse.length := by exact Eq.symm length_reverse
       rw [aux5] at aux4
-      have aux2:(zipWith Nat.pair (tail.reverse ++ [head]) (n2l l2N)) = (zipWith Nat.pair tail.reverse (n2l l2N)) := by simp [c_list_zip_evp_aux_2 aux4]
+      have aux2:(zipWith f (tail.reverse ++ [head]) (n2l l2N)) = (zipWith f tail.reverse (n2l l2N)) := by simp [c_list_zipWith_evp_aux_2 aux4]
       rw [aux2]
-    sorry
-    · have omwv: ∃ head2 list2, drop tail.length (n2l l2N) = head2::list2 := by exact ne_nil_iff_exists_cons.mp hh
+    -- sorry
+    · -- this is the case where l2N is longer than l1N.
+      have omwv: ∃ head2 list2, drop tail.length (n2l l2N) = head2::list2 := by exact ne_nil_iff_exists_cons.mp hh
       rcases omwv with ⟨head2,list2,hl2⟩
       simp only [hl2]
-      have main : (Nat.pair head (head2 :: list2).headI :: (zipWith Nat.pair tail.reverse (n2l l2N)).reverse) = (zipWith Nat.pair (tail.reverse ++ [head]) (n2l l2N)).reverse := by
+
+      have main : (f head (head2 :: list2).headI :: (zipWith f tail.reverse (n2l l2N)).reverse) = (zipWith f (tail.reverse ++ [head]) (n2l l2N)).reverse := by
         simp
-        have aux := length_lt_of_drop_ne_nil hh
-        have aux2 : ((tail.reverse ++ [head])).length ≤ (n2l l2N).length := by grind
+        have aux1 := length_lt_of_drop_ne_nil hh
         have aux3 : (n2l l2N) = (take tail.length (n2l l2N)) ++ drop tail.length (n2l l2N) := by
           exact Eq.symm (take_append_drop tail.length (n2l l2N))
-        have aux4 : (n2l l2N) = (take tail.length (n2l l2N)) ++ (head2::list2) := by grind only
-        have aux5 : (n2l l2N) = ((take tail.length (n2l l2N)) ++ [head2]) ++ list2 := by grind
-        have aux6 :(tail.reverse ++ [head]).length = (take tail.length (n2l l2N) ++ [head2]).length := by grind
+        have aux5 : (n2l l2N) = (take tail.length (n2l l2N)) ++ [head2] ++ list2 := by
+          rw (config:={occs:=.pos [1]}) [aux3]
+          rw [append_assoc]
+          simp [hl2]
+
         have aux7 :
           let l₁:=tail.reverse ++ [head]
           let l₂:=take tail.length (n2l l2N) ++ [head2] ++ list2
-          let l₁':=zipWith Nat.pair (tail.reverse) (take tail.length (n2l l2N))
-          let l₂':List ℕ :=[Nat.pair head head2]
-          let f:= Nat.pair
+          let l₁':=zipWith f (tail.reverse) (take tail.length (n2l l2N))
+          let l₂':List ℕ :=[f head head2]
+          -- let f:= f
           ∃ ws xs ys zs, ws.length = ys.length ∧ l₁ = ws ++ xs ∧ l₂ = ys ++ zs ∧ l₁' = zipWith f ws ys ∧ l₂' = zipWith f xs zs := by
             let ws := tail.reverse
             let ys := take tail.length (n2l l2N)
@@ -562,7 +566,8 @@ theorem c_list_zip_evp_aux_2P {a b : List ℕ} {f:ℕ→ℕ→ℕ} (h:a.length�
             let zs := [head2] ++ list2
             use ws,xs,ys,zs
             constructor
-            · grind
+            · simp [ws,ys]
+              exact le_of_succ_le aux1
             · constructor
               · exact rfl
               · constructor
@@ -571,64 +576,22 @@ theorem c_list_zip_evp_aux_2P {a b : List ℕ} {f:ℕ→ℕ→ℕ} (h:a.length�
                   · exact rfl
                   · exact rfl
         have aux8 := zipWith_eq_append_iff.mpr aux7
-        
+
         rw (config:={occs:=.pos [2]}) [aux5]
         rw [aux8]
         simp
         rw (config:={occs:=.pos [1]}) [aux5]
-        have aux10: (take tail.length (n2l l2N) ++ [head2] ++ list2) = (take tail.length (n2l l2N) ++ ([head2] ++ list2)) := by exact append_assoc (take tail.length (n2l l2N)) [head2] list2
-        have aux9 : tail.reverse.length = (take tail.length (n2l l2N)).length := by grind
-        rw [aux10]
-        #check @zipWith_append ℕ ℕ ℕ Nat.pair tail.reverse [] (take tail.length (n2l l2N)) ([head2] ++ list2)
-        -- exact @zipWith_append ℕ ℕ ℕ Nat.pair tail.reverse [] (take tail.length (n2l l2N)) ([head2] ++ list2) aux9
-        have aux11 := @zipWith_append ℕ ℕ ℕ Nat.pair tail.reverse [] (take tail.length (n2l l2N)) ([head2] ++ list2) aux9
-        simp at aux11
-        exact aux11
+        rw [append_assoc (take tail.length (n2l l2N)) [head2] list2]
+
+        have aux9 : tail.reverse.length ≤ (take tail.length (n2l l2N)).length := by
+          simp
+          exact le_of_succ_le aux1
+        exact  c_list_zipWith_evp_aux_1 aux9
       rw [main]
-      
-        
-        
-        
-        
-      -- simp only [hh]
-      
-      
-      
-      simp
-    
-    -- simp [asd, -encode_list_cons, -encode_list_nil] at ih
-    -- simp_all [asd, -encode_list_cons, -encode_list_nil]
-    
-    
-    -- simp only [ih]
-    
-  -- simp only [foldl_cons, pair_r, pair_l, length_cons]
-  -- simp only [ofNat_encode]
-  -- simp [ih]
-  -- simp only [encode_list_cons, encode_nat, encode_ofNat, succ_eq_add_one, encode_list_nil]
-  -- simp only [ih]
-  -- simp [-encode_list_cons, -encode_list_nil]
-    exact ih
-  
 
-
-    constructor
-    · sorry
-    · 
-
-
-
-    induction (n2l l2N) with
-    | nil =>
-      simp [ih, -encode_list_cons, -encode_list_nil]
-    | cons head2 tail2 ih2 => sorry
-    simp [ih, -encode_list_cons, -encode_list_nil]
-
-
-
--- @[simp] theorem c_list_zip_ev : eval O (c_list_zip cf) lN = l2n ((n2l lN).map (eval_prim O cf)) := by simp [← eval_prim_eq_eval c_list_zip_ev_pr]
+-- @[simp] theorem c_list_zipWith_ev : eval O (c_list_zipWith cf) lN = l2n ((n2l lN).map (eval_prim O cf)) := by simp [← eval_prim_eq_eval c_list_zipWith_ev_pr]
 end Nat.RecursiveIn.Code
-end list_zip
+end list_zipWith
 
 section list_map'
 namespace Nat.RecursiveIn.Code
